\documentclass{article}
\usepackage{amsmath}
\usepackage{amsfonts}
\usepackage{amssymb}
\usepackage[margin=0.5in]{geometry}
\usepackage[normalem]{ulem}
\usepackage{graphicx} % Required for inserting images
\usepackage{mathtools}
\usepackage{enumitem}
\usepackage[export]{adjustbox}


\newcommand{\ceil}[1]{\lceil #1 \rceil}
\newcommand{\If}[1]{\textrm{ if #1}}
\newcommand{\then}[1]{\textrm{ then #1}}
\newcommand{\ForAll}[0]{\textrm{ for all }}
\newcommand{\Let}[0]{\textrm{Let }}
\newcommand{\proof}[1]{\textbf{Proof: #1}}
\newcommand{\counter}[1]{\textbf{Counterexample: #1}}
\newcommand{\ns}[1]{\mathbb{#1}}
\newcommand{\Reals}[0]{\ns{R}}
\newcommand{\lub}[1]{\text{lub$_{#1}$}}
\newcommand{\glb}[1]{\text{glb$_{#1}$}}
\newcommand{\pointspace}[3]{\langle#1, #2, #3\rangle}
\newcommand{\pointplane}[2]{\langle#1, #2\rangle}
\newcommand{\inte}[0]{\text{int}}

\newcommand{\set}[1]{\{#1\}}
\newcommand{\osset}{\mathrel{\ooalign{$\subseteq$\cr
  \hidewidth\raise.225ex\hbox{$\circ\mkern.5mu$}\cr}}}
\newcommand{\csset}{\mathrel{\ooalign{$\subseteq$\cr
  \hidewidth\raise.225ex\hbox{$\bullet\mkern.5mu$}\cr}}}
  
\newcommand{\pr}[1]{\operatorname{P}(#1)}

\title{\MakeUppercase{\jobname}}
\author{Justin Nguyen}
\date{\today}

\begin{document}
\maketitle

\begin{enumerate}
  \item $9\cdot 10^6 = 9,000,000$ seven-digit phone numbers. %because 9 choices for the first number, and 10 choices each for the next 6.
  \item \begin{enumerate}
    \item $8! = 40320$ seatings %which is all arrangements 8 people.
    \item $5!\cdot 4 \cdot 3! = 2880$ consecutive male seatings. %because there are $5!$ ways the men can sit
    \item $4!\cdot 2^4 = 384$ consecutive couples seatings. %the arrangements of the couples by their swaps
  \end{enumerate}
  \item $6m, 7s, 4e \to 2$ books
  \begin{enumerate}
    \item $\binom{6}{2} + \binom{7}{2} + \binom{4}{2} = 42$ choices of the two books who share the same subject. %sum of choosing 2 at a time from each book set
    \item $\binom{6}{1}\binom{7}{1} + \binom{6}{1}\binom{4}{1} + \binom{7}{1}\binom{4}{1} = 94$ choices of two books who don't share the same subject. %sum of products of choosing two books from each set
  \end{enumerate}
  \item $8w, 6m \to 3w, 3m$
  \begin{enumerate}
    \item $\binom{8}{3}[\binom{6}{3} - \binom{4}{1}] = 896$ committees where $m_1, m_2$ don't work together.
    \item $\binom{6}{3}[\binom{8}{3} - \binom{6}{1}] = 1000$ committees where $w_1, w_2$ don't work together.
    \item $\binom{8}{3}\binom{6}{3} - P^7_3 = 910$ committees where $w_1, m_1$ don't work together.%P^7_3 = committees where w1,m1 work together
    \footnote{$P^7_3$ is a simplification of the number of committees where $w_1, m_1$ work together.}
  \end{enumerate}
  \item Let $D_6 = \set{1,2,3,4,5,6},A =$ rolling $1\ldots 6$ in any order, and $|S| = |D_6|^6$.\\
  If the point $r_1 = (1,2,3,4,5,6) \in A \implies$other points in $A$ must be arrangements of $r_1 \implies |A| = |D_6|!$\\
  $\therefore \pr{A} = \frac{6!}{6^6} \approx 0.015$
  \item $|S| = \binom{10}{5}, |A| = \binom{6}{5} \implies \pr{A} = \frac{|A|}{|S|} \approx 0.02$
  \item 
  \item $52$ cards $\to$ 5 cards; $|S| = \binom{52}{5}$ \begin{enumerate}
    \item $\pr{3A, 2K} = \frac{\binom{4}{3}\binom{4}{2}}{\binom{52}{5}} \approx 0.000009$
    \item $\pr{3R_n, 2R_k} = $ TODO
  \end{enumerate}
  \item $2w, 4h, 7a \to 1w, 2h, 3a$\\
  $|S| = P^{13}_6$
  \item \begin{enumerate}
    \item Fluke $=\binom{5}{1}\binom{4}{1}\binom{3}{1}\binom{2}{1}\binom{1}{1} = 120$ arrangements.
    \item Propose $= \binom{7}{2}\binom{5}{1}\binom{4}{2}\binom{2}{1}\binom{1}{1} = 1260$ arrangements.
    \item Mississippi = $\binom{11}{1}\binom{10}{4}\binom{6}{4}\binom{2}{2} = 34650$ arrangements.
  \end{enumerate}
  \item 11
  \item 12
  
  \newpage
  \item \proof{}$\sum_{k=0}^{n}\binom{n}{k} = 2^n$\\
  The Binomial Theorem states that $(x+y)^n = \sum_{k=0}^{n}\binom{n}{k}x^{n-k}y^k$.\\
  Then, let $x=y=1 \implies (1+1)^n = \sum_{k=0}^{n}\binom{n}{k}1^{n-k}1^k = \sum_{k=0}^{n}\binom{n}{k}1^n = \sum_{k=0}^{n}\binom{n}{k}$.\\
  $\therefore 2^n = \sum_{k=0}^{n}\binom{n}{k}$.
  
  \item \proof{} $\sum_{k=0}^{n>0}(-1)^k\binom{n}{k} = 0$\\
  \textbf{Case} $n=1$:\\
  \[\sum_{k=0}^{1}(-1)^k\binom{1}{k} = (-1)^0\binom{1}{0} + (-1)^1\binom{1}{1} = 0\]
  
  \textbf{Case} $n = n + 1$:\\
  Note that $(\forall \alpha, \beta \in\ns{N})$ and $\alpha \geq \beta$
  \begin{itemize}
    \item $\binom{\alpha}{0} = \binom{\alpha}{\alpha} = 1$
    \item $\binom{\alpha}{1} = \binom{\alpha}{\alpha - 1} = \alpha$
    \item $\binom{\alpha}{\beta} = \binom{\alpha}{\alpha - \beta}$
  \end{itemize}
  Assume that $\sum_{k=0}^{n>0}(-1)^k\binom{n}{k} = 0$. Then $n+1$ is:
  \[\sum_{k=0}^{n+1}(-1)^k\binom{n+1}{k} =\]

  \[(-1)^0\binom{n+1}{0} + (-1)^1\binom{n+1}{1} + 
  \ldots + (-1)^{n+1-k}\binom{n+1}{n+1-k} + \ldots + (-1)^k\binom{n+1}{k} + \ldots +
  (-1)^{n}\binom{n+1}{n} + (-1)^{n+1}\binom{n+1}{n + 1}\]\\
  We rearrange the terms.
  \[(-1)^0\binom{n+1}{0} + (-1)^{n+1}\binom{n+1}{n+1}  + \ldots
  + (-1)^{n+1-k}\binom{n+1}{n+1-k} + (-1)^k\binom{n+1}{k} + \ldots
  + (-1)^1\binom{n+1}{1} + (-1)^n\binom{n+1}{n}\]
\end{enumerate}

\end{document}